coq/examples/chacha20.v
@@ -5,270 +5,202 @@ Section chacha20.
 Open Scope Z_scope.
 Open Scope bool_scope.
 Open Scope hacspec_scope.
-
-
-
+Require Import Hacspec.Lib.
 
 Definition state := nseq (uint32) (usize 16).
 
 Definition state_idx :=
   nat_mod (usize 16).
-  
 Definition uint_size_in_state_idx(n : uint_size) : state_idx := int_in_nat_mod n.
 Coercion uint_size_in_state_idx : uint_size >-> state_idx.
 
-Definition state_bytes := nseq (uint8) (usize 64).
+Definition constants := nseq (uint32) (usize 4).
 
-Definition iv := nseq (uint8) (usize 12).
+Definition constants_idx :=
+  nat_mod (usize 4).
+Definition uint_size_in_constants_idx(n : uint_size) : constants_idx := int_in_nat_mod n.
+Coercion uint_size_in_constants_idx : uint_size >-> constants_idx.
 
-Definition key := nseq (uint8) (usize 32).
+Definition block := nseq (uint8) (usize 64).
 
-Definition state_to_bytes (x_0 : state) : state_bytes :=
-  let r_1 := array_new_ (secret (repr 0)) (64) in
-  let r_1 :=
-    foldi (usize 0) (array_len (x_0)) (fun i_2 r_1 =>
-      let bytes_3 := uint32_to_be_bytes (array_index (x_0) (i_2)) in
-      let r_1 :=
-        array_upd r_1 ((i_2) * (usize 4)) (array_index (bytes_3) (usize 3))
-      in
-      let r_1 :=
-        array_upd r_1 (((i_2) * (usize 4)) + (usize 1)) (
-          array_index (bytes_3) (usize 2))
-      in
-      let r_1 :=
-        array_upd r_1 (((i_2) * (usize 4)) + (usize 2)) (
-          array_index (bytes_3) (usize 1))
-      in
-      let r_1 :=
-        array_upd r_1 (((i_2) * (usize 4)) + (usize 3)) (
-          array_index (bytes_3) (usize 0))
-      in
-      (r_1))
-    r_1
-  in
-  r_1.
+Definition cha_cha_iv := nseq (uint8) (usize 12).
 
-Definition chacha_line
-  (a_4 : state_idx)
-  (b_5 : state_idx)
-  (d_6 : state_idx)
-  (s_7 : uint_size)
-  (m_8 : state)
+Definition cha_cha_key := nseq (uint8) (usize 32).
+
+Definition chacha20_line
+  (a_0 : state_idx)
+  (b_1 : state_idx)
+  (d_2 : state_idx)
+  (s_3 : uint_size)
+  (m_4 : state)
   : state :=
-  let state_9 := m_8 in
-  let state_9 :=
-    array_upd state_9 (a_4) (
-      (array_index (state_9) (a_4)) .+ (array_index (state_9) (b_5)))
+  let state_5 := m_4 in
+  let state_5 :=
+    array_upd state_5 (a_0) (
+      (array_index (state_5) (a_0)) .+ (array_index (state_5) (b_1)))
   in
-  let state_9 :=
-    array_upd state_9 (d_6) (
-      (array_index (state_9) (d_6)) .^ (array_index (state_9) (a_4)))
+  let state_5 :=
+    array_upd state_5 (d_2) (
+      (array_index (state_5) (d_2)) .^ (array_index (state_5) (a_0)))
   in
-  let state_9 :=
-    array_upd state_9 (d_6) (
-      uint32_rotate_left (array_index (state_9) (d_6)) (s_7))
+  let state_5 :=
+    array_upd state_5 (d_2) (
+      uint32_rotate_left (array_index (state_5) (d_2)) (s_3))
   in
-  state_9.
+  state_5.
 
-Definition chacha_quarter_round
-  (a_10 : state_idx)
-  (b_11 : state_idx)
-  (c_12 : state_idx)
-  (d_13 : state_idx)
-  (state_14 : state)
+Definition chacha20_quarter_round
+  (a_6 : state_idx)
+  (b_7 : state_idx)
+  (c_8 : state_idx)
+  (d_9 : state_idx)
+  (state_10 : state)
   : state :=
-  let state_15 := chacha_line (a_10) (b_11) (d_13) (usize 16) (state_14) in
-  let state_16 := chacha_line (c_12) (d_13) (b_11) (usize 12) (state_15) in
-  let state_17 := chacha_line (a_10) (b_11) (d_13) (usize 8) (state_16) in
-  chacha_line (c_12) (d_13) (b_11) (usize 7) (state_17).
+  let state_11 := chacha20_line (a_6) (b_7) (d_9) (usize 16) (state_10) in
+  let state_12 := chacha20_line (c_8) (d_9) (b_7) (usize 12) (state_11) in
+  let state_13 := chacha20_line (a_6) (b_7) (d_9) (usize 8) (state_12) in
+  chacha20_line (c_8) (d_9) (b_7) (usize 7) (state_13).
 
-Definition chacha_double_round (state_18 : state) : state :=
+Definition chacha20_double_round (state_14 : state) : state :=
+  let state_15 :=
+    chacha20_quarter_round (usize 0) (usize 4) (usize 8) (usize 12) (state_14)
+  in
+  let state_16 :=
+    chacha20_quarter_round (usize 1) (usize 5) (usize 9) (usize 13) (state_15)
+  in
+  let state_17 :=
+    chacha20_quarter_round (usize 2) (usize 6) (usize 10) (usize 14) (state_16)
+  in
+  let state_18 :=
+    chacha20_quarter_round (usize 3) (usize 7) (usize 11) (usize 15) (state_17)
+  in
   let state_19 :=
-    chacha_quarter_round (usize 0) (usize 4) (usize 8) (usize 12) (state_18)
+    chacha20_quarter_round (usize 0) (usize 5) (usize 10) (usize 15) (state_18)
   in
   let state_20 :=
-    chacha_quarter_round (usize 1) (usize 5) (usize 9) (usize 13) (state_19)
+    chacha20_quarter_round (usize 1) (usize 6) (usize 11) (usize 12) (state_19)
   in
   let state_21 :=
-    chacha_quarter_round (usize 2) (usize 6) (usize 10) (usize 14) (state_20)
+    chacha20_quarter_round (usize 2) (usize 7) (usize 8) (usize 13) (state_20)
   in
-  let state_22 :=
-    chacha_quarter_round (usize 3) (usize 7) (usize 11) (usize 15) (state_21)
-  in
-  let state_23 :=
-    chacha_quarter_round (usize 0) (usize 5) (usize 10) (usize 15) (state_22)
-  in
-  let state_24 :=
-    chacha_quarter_round (usize 1) (usize 6) (usize 11) (usize 12) (state_23)
-  in
-  let state_25 :=
-    chacha_quarter_round (usize 2) (usize 7) (usize 8) (usize 13) (state_24)
-  in
-  chacha_quarter_round (usize 3) (usize 4) (usize 9) (usize 14) (state_25).
+  chacha20_quarter_round (usize 3) (usize 4) (usize 9) (usize 14) (state_21).
 
-Definition chacha20_constants_init  : seq uint32 :=
-  let constants_26 := seq_new_ (secret (repr 0)) (usize 4) in
-  let constants_26 :=
-    array_upd constants_26 (usize 0) (secret (repr 1634760805))
+Definition chacha20_rounds (state_22 : state) : state :=
+  let st_23 := state_22 in
+  let st_23 :=
+    foldi (usize 0) (usize 10) (fun i_24 st_23 =>
+      let st_23 := chacha20_double_round (st_23) in
+      (st_23))
+    st_23
   in
-  let constants_26 :=
-    array_upd constants_26 (usize 1) (secret (repr 857760878))
-  in
-  let constants_26 :=
-    array_upd constants_26 (usize 2) (secret (repr 2036477234))
-  in
-  let constants_26 :=
-    array_upd constants_26 (usize 3) (secret (repr 1797285236))
-  in
-  constants_26.
+  st_23.
 
-Definition chacha20_key_to_u32s (key_27 : key) : seq uint32 :=
-  let uints_28 := seq_new_ (secret (repr 0)) (usize 8) in
-  let uints_28 :=
-    array_upd uints_28 (usize 0) (
-      uint32_from_le_bytes (
-        array_from_slice_range (secret (repr 0)) (4) (key_27) (
-          (usize 0, usize 4))))
+Definition chacha20_core (ctr_25 : uint32) (st0_26 : state) : state :=
+  let state_27 := st0_26 in
+  let state_27 :=
+    array_upd state_27 (usize 12) (
+      (array_index (state_27) (usize 12)) .+ (ctr_25))
   in
-  let uints_28 :=
-    array_upd uints_28 (usize 1) (
-      uint32_from_le_bytes (
-        array_from_slice_range (secret (repr 0)) (4) (key_27) (
-          (usize 4, usize 8))))
-  in
-  let uints_28 :=
-    array_upd uints_28 (usize 2) (
-      uint32_from_le_bytes (
-        array_from_slice_range (secret (repr 0)) (4) (key_27) (
-          (usize 8, usize 12))))
-  in
-  let uints_28 :=
-    array_upd uints_28 (usize 3) (
-      uint32_from_le_bytes (
-        array_from_slice_range (secret (repr 0)) (4) (key_27) (
-          (usize 12, usize 16))))
-  in
-  let uints_28 :=
-    array_upd uints_28 (usize 4) (
-      uint32_from_le_bytes (
-        array_from_slice_range (secret (repr 0)) (4) (key_27) (
-          (usize 16, usize 20))))
-  in
-  let uints_28 :=
-    array_upd uints_28 (usize 5) (
-      uint32_from_le_bytes (
-        array_from_slice_range (secret (repr 0)) (4) (key_27) (
-          (usize 20, usize 24))))
-  in
-  let uints_28 :=
-    array_upd uints_28 (usize 6) (
-      uint32_from_le_bytes (
-        array_from_slice_range (secret (repr 0)) (4) (key_27) (
-          (usize 24, usize 28))))
-  in
-  let uints_28 :=
-    array_upd uints_28 (usize 7) (
-      uint32_from_le_bytes (
-        array_from_slice_range (secret (repr 0)) (4) (key_27) (
-          (usize 28, usize 32))))
-  in
-  uints_28.
+  let k_28 := chacha20_rounds (state_27) in
+  (k_28) array_add (state_27).
 
-Definition chacha20_iv_to_u32s (iv_29 : iv) : seq uint32 :=
-  let uints_30 := seq_new_ (secret (repr 0)) (usize 3) in
-  let uints_30 :=
-    array_upd uints_30 (usize 0) (
-      uint32_from_le_bytes (
-        array_from_slice_range (secret (repr 0)) (4) (iv_29) (
-          (usize 0, usize 4))))
+Definition chacha20_constants_init  : constants :=
+  let constants_29 := array_new_ (secret (repr 0)) (4) in
+  let constants_29 :=
+    array_upd constants_29 (usize 0) (secret (repr 1634760805))
   in
-  let uints_30 :=
-    array_upd uints_30 (usize 1) (
-      uint32_from_le_bytes (
-        array_from_slice_range (secret (repr 0)) (4) (iv_29) (
-          (usize 4, usize 8))))
+  let constants_29 :=
+    array_upd constants_29 (usize 1) (secret (repr 857760878))
   in
-  let uints_30 :=
-    array_upd uints_30 (usize 2) (
-      uint32_from_le_bytes (
-        array_from_slice_range (secret (repr 0)) (4) (iv_29) (
-          (usize 8, usize 12))))
+  let constants_29 :=
+    array_upd constants_29 (usize 2) (secret (repr 2036477234))
   in
-  uints_30.
+  let constants_29 :=
+    array_upd constants_29 (usize 3) (secret (repr 1797285236))
+  in
+  constants_29.
 
-Definition chacha20_ctr_to_seq (ctr_31 : uint32) : seq uint32 :=
-  let uints_32 := seq_new_ (secret (repr 0)) (usize 1) in
-  let uints_32 := array_upd uints_32 (usize 0) (ctr_31) in
-  uints_32.
-
-Definition chacha_block_init
-  (key_33 : key)
-  (ctr_34 : uint32)
-  (iv_35 : iv)
+Definition chacha20_init
+  (key_30 : cha_cha_key)
+  (iv_31 : cha_cha_iv)
+  (ctr_32 : uint32)
   : state :=
-  array_from_seq (16) (
-    seq_concat (
-      seq_concat (
-        seq_concat (chacha20_constants_init ) (chacha20_key_to_u32s (key_33))) (
-        chacha20_ctr_to_seq (ctr_34))) (chacha20_iv_to_u32s (iv_35))).
+  let st_33 := array_new_ (secret (repr 0)) (16) in
+  let st_33 := array_update (st_33) (usize 0) (chacha20_constants_init ) in
+  let st_33 := array_update (st_33) (usize 4) (array_to_le_uint32s (key_30)) in
+  let st_33 := array_upd st_33 (usize 12) (ctr_32) in
+  let st_33 := array_update (st_33) (usize 13) (array_to_le_uint32s (iv_31)) in
+  st_33.
 
-Definition chacha_block_inner
-  (key_36 : key)
-  (ctr_37 : uint32)
-  (iv_38 : iv)
-  : state :=
-  let st_39 := chacha_block_init (key_36) (ctr_37) (iv_38) in
-  let state_40 := st_39 in
-  let state_40 :=
-    foldi (usize 0) (usize 10) (fun i_41 state_40 =>
-      let state_40 := chacha_double_round (state_40) in
-      (state_40))
-    state_40
-  in
-  let state_40 :=
-    foldi (usize 0) (usize 16) (fun i_42 state_40 =>
-      let state_40 :=
-        array_upd state_40 (i_42) (
-          (array_index (state_40) (i_42)) .+ (array_index (st_39) (i_42)))
-      in
-      (state_40))
-    state_40
-  in
-  state_40.
+Definition chacha20_key_block (state_34 : state) : block :=
+  let state_35 := chacha20_core (secret (repr 0)) (state_34) in
+  array_from_seq (64) (array_to_le_bytes (state_35)).
 
-Definition chacha_block
-  (key_43 : key)
-  (ctr_44 : uint32)
-  (iv_45 : iv)
-  : state_bytes :=
-  let state_46 := chacha_block_inner (key_43) (ctr_44) (iv_45) in
-  state_to_bytes (state_46).
+Definition chacha20_key_block0
+  (key_36 : cha_cha_key)
+  (iv_37 : cha_cha_iv)
+  : block :=
+  let state_38 := chacha20_init (key_36) (iv_37) (secret (repr 0)) in
+  chacha20_key_block (state_38).
 
-Definition chacha (key_47 : key) (iv_48 : iv) (m_49 : byte_seq) : byte_seq :=
-  let ctr_50 := secret (repr 1) in
-  let blocks_out_51 := seq_new_ (secret (repr 0)) (seq_len (m_49)) in
-  let '(ctr_50, blocks_out_51) :=
-    foldi (usize 0) (seq_num_chunks (m_49) (usize 64)) (fun i_52 '(
-        ctr_50,
-        blocks_out_51
-      ) =>
-      let '(block_len_53, msg_block_54) :=
-        seq_get_chunk (m_49) (usize 64) (i_52)
-      in
-      let key_block_55 := chacha_block (key_47) (ctr_50) (iv_48) in
-      let msg_block_padded_56 := array_new_ (secret (repr 0)) (64) in
-      let msg_block_padded_57 :=
-        array_update_start (msg_block_padded_56) (msg_block_54)
+Definition chacha20_encrypt_block
+  (st0_39 : state)
+  (ctr_40 : uint32)
+  (plain_41 : block)
+  : block :=
+  let st_42 := chacha20_core (ctr_40) (st0_39) in
+  let pl_43 := array_from_seq (16) (array_to_le_uint32s (plain_41)) in
+  let st_44 := (pl_43) array_xor (st_42) in
+  array_from_seq (64) (array_to_le_bytes (st_44)).
+
+Definition chacha20_encrypt_last
+  (st0_45 : state)
+  (ctr_46 : uint32)
+  (plain_47 : byte_seq)
+  : byte_seq :=
+  let b_48 := array_new_ (secret (repr 0)) (64) in
+  let b_48 := array_update (b_48) (usize 0) (plain_47) in
+  let b_48 := chacha20_encrypt_block (st0_45) (ctr_46) (b_48) in
+  array_slice (b_48) (usize 0) (seq_len (plain_47)).
+
+Definition chacha20_update (st0_49 : state) (m_50 : byte_seq) : byte_seq :=
+  let blocks_out_51 := seq_new_ (secret (repr 0)) (seq_len (m_50)) in
+  let n_blocks_52 := seq_num_exact_chunks (m_50) (usize 64) in
+  let blocks_out_51 :=
+    foldi (usize 0) (n_blocks_52) (fun i_53 blocks_out_51 =>
+      let msg_block_54 := seq_get_exact_chunk (m_50) (usize 64) (i_53) in
+      let b_55 :=
+        chacha20_encrypt_block (st0_49) (secret (pub_u32 (i_53))) (
+          array_from_seq (64) (msg_block_54))
       in
       let blocks_out_51 :=
-        seq_set_chunk (blocks_out_51) (usize 64) (i_52) (
-          array_slice_range (
-            (msg_block_padded_57) array_xor_.^ (key_block_55)) (
-            (usize 0, block_len_53)))
+        seq_set_exact_chunk (blocks_out_51) (usize 64) (i_53) (b_55)
       in
-      let ctr_50 := (ctr_50) .+ (secret (repr 1)) in
-      (ctr_50, blocks_out_51))
-    (ctr_50, blocks_out_51)
+      (blocks_out_51))
+    blocks_out_51
+  in
+  let last_block_56 := seq_get_remainder_chunk (m_50) (usize 64) in
+  let '(blocks_out_51) :=
+    if (seq_len (last_block_56)) !=.? (usize 0) then (
+      let b_57 :=
+        chacha20_encrypt_last (st0_49) (secret (pub_u32 (n_blocks_52))) (
+          last_block_56)
+      in
+      let blocks_out_51 :=
+        seq_set_chunk (blocks_out_51) (usize 64) (n_blocks_52) (b_57)
+      in
+      (blocks_out_51)
+    ) else ( (blocks_out_51)
+    )
   in
   blocks_out_51.
+
+Definition chacha20
+  (key_58 : cha_cha_key)
+  (iv_59 : cha_cha_iv)
+  (ctr_60 : int32)
+  (m_61 : byte_seq)
+  : byte_seq :=
+  let state_62 := chacha20_init (key_58) (iv_59) (secret (ctr_60)) in
+  chacha20_update (state_62) (m_61).
 
